

# Module 2

## Successive Differentiation, Expansion Of Functions, Indeterminate Forms

### 2.1 Successive differentiation

# Module 2

2	<b>Successive Differentiation, Expansion Of Functions, Indeterminate Forms</b>	
	2.1	Successive differentiation: nth derivative of standard functions. Leibnitz's Theorem (without proof) and problems.
	2.2	Taylor's Theorem (only statement) and Taylor's series, Maclaurin's series(only Statement) Expansion of $e^x$ , $\sin x$ , $\cos x$ , $\tan x$
		<b>#Self-learning topic:</b> Expansion of $\sinh(x)$ , $\cosh(x)$ , $\tanh(x)$ , $\log(1+x)$ , Indeterminate forms, L'Hospital Rule, problems involving series

# Successive Differentiation

❖ If  $y = f(x)$  then

- first derivative of  $f(x)$  is denoted by  $f'(x)$  or  $y_1$
- Second derivative of  $f(x)$  is denoted by  $f''(x)$  or  $y_2$
- Similarly nth derivative of  $f(x)$  is denoted by  $f^{(n)}(x)$  or  $y_n$

❖ nth Derivative of  $f(x)$  at  $x = a$  is denoted by

$$f^{(n)}(a) = f^n(a) = \left[ \frac{d^n y}{dx^n} \right] \text{ at } x = a$$

❖ If  $y = x^m$  then

$$y_1 = mx^{m-1}$$

$$y_2 = m(m-1)x^{m-2}$$

$$y_3 = m(m-1)(m-2)x^{m-3}$$

$$y_n = m(m-1)(m-2) \dots (m-n)x^{m-n} \quad \text{where } n < m$$

$$= m(m-1)(m-2) \dots 3.2.1 x^{m-m} = m! \quad \text{if } n = m$$

$$= 0 \quad \text{where } n > m$$

❖ If  $y = (ax + b)^m$  then

$$y_n = m(m-1)(m-2) \dots (m-n+1)a^n(ax+b)^{m-n}; \text{if } n < m$$

$$= m! a^n \quad ; \text{if } m = n$$

$$= 0 \quad ; \text{if } n > m$$

# Remember

Sr. No	$y = f(x)$	$y_n$
1	$(ax+b)^m$	$= m(m-1)(m-2)\cdots(m-n+1)a^n (ax+b)^{m-n}$ if $n < m$
2	$(ax+b)^{-m}$	$= (-1)^n m(m+1)(m+2)\cdots(m+n-1)a^n (ax+b)^{-m-n}$ $= (-1)^n \cdot \frac{(m+n-1)!}{(m-1)!} \cdot \frac{a^n}{(ax+b)^{m+n}}$
3	$x^m$	$= m(m-1)(m-2)\cdots(m-n+1)x^{m-n}$ if $n < m$
4	$1/x^m$	$= (-1)^n \cdot \frac{(m+n-1)!}{(m-1)!} \cdot \frac{1}{(x)^{m+n}}$

# Remember

Sr. No	$y = f(x)$	$y_n$
4	$\frac{1}{(ax+b)}$	$= \frac{(-1)^n \cdot n! a^n}{(ax+b)^{n+1}}$
5	$\log(ax+b)$	$= \frac{(-1)^{n-1} \cdot (n-1)! a^n}{(ax+b)^n}$
6	$a^{mx}$	$= m^n a^{mx} (\log a)^n$
7	$e^{mx}$	$= m^n e^{mx}$

# Remember

Sr. No	$y = f(x)$	$y_n$
8	$\sin(ax+b)$	$= a^n \sin\left(ax+b+\frac{n\pi}{2}\right)$
9	$\cos(ax+b)$	$= a^n \cos\left(ax+b+\frac{n\pi}{2}\right)$
10	$e^{ax} \sin(bx+c)$	$= r^n e^{ax} \sin(bx+c+n\phi)$ where $r = \sqrt{a^2+b^2}$ & $\phi = \tan^{-1}\left(\frac{b}{a}\right)$
11	$e^{ax} \cos(bx+c)$	$= r^n e^{ax} \cos(bx+c+n\phi)$ where $r = \sqrt{a^2+b^2}$ & $\phi = \tan^{-1}\left(\frac{b}{a}\right)$

# Remember

Sr. No	$y = f(x)$	$y_n$
12	$k^x \sin(bx + c)$	$= r^n k^x \sin(bx + c + n\phi)$ where $r = \sqrt{(\log k)^2 + b^2}$ & $\phi = \tan^{-1}\left(\frac{b}{\log k}\right)$
13	$k^x \cos(bx + c)$	$= r^n k^x \cos(bx + c + n\phi)$ where $r = \sqrt{(\log k)^2 + b^2}$ & $\phi = \tan^{-1}\left(\frac{b}{\log k}\right)$



# Example:1

❖ If  $y = \frac{1}{1+x+x^2+x^3}$  then find  $y_n$

❖ Solution



**SOMAIYA**  
VIDYAVIHAR UNIVERSITY

K J Somaia College of Engineering



## Example:2

❖ If  $y = \frac{8x}{x^3 - 2x^2 - 4x + 8}$  then find  $y_n$

❖ **Solution**

$$\text{If } v = \frac{1}{(x-2)^2}, \quad v_n = \frac{(-1)^n (n+1)! (1)^n}{(x-2)^{n+2}}$$

$$\text{If } w = \frac{1}{x+2}, \quad w_n = \frac{(-1)^n n! (1)^n}{(x+2)^n}$$

$$\therefore y_n = \frac{(-1)^n n!}{(x-2)^{n+1}} + 4 \cdot \frac{(-1)^n (n+1)!}{(x-2)^{n+2}} - \frac{(-1)^n}{(x+2)^n}.$$

## Example:3

❖ If  $y = \frac{x}{(x+1)^4}$ , find  $y_n$ .

❖ Solution:  $y = \frac{x}{(x+1)^4} = \frac{(x+1) - 1}{(x+1)^4}$

$$\begin{aligned}
 \therefore y_n &= \frac{(-1)^n (n+2)!}{2!(x+1)^{n+3}} - \frac{(-1)^n (n+3)!}{3!(x+1)^{n+4}} \\
 &= \frac{(-1)^n (n+2)!}{6(x+1)^{n+3}} \left[ 3 - \frac{(n+3)}{(x+1)} \right] \\
 &= \frac{(-1)^n (n+2)!}{6(x+1)^{n+4}} (3x - n).
 \end{aligned}$$

## Example:4

❖ If  $y = x \log \left( \frac{x-1}{x+1} \right)$ , prove that

$$y_n = (-1)^{n-2} (n-2)! \left[ \frac{x-n}{(x-1)^n} - \frac{x+n}{(x+1)^n} \right].$$

❖ **Solution:** We have  $y = x \log (x-1) - x \log (x+1)$

$$\therefore y_1 = \frac{x}{x-1} + \log(x-1) - \frac{x}{x+1} - \log(x+1)$$

$$= \log(x-1) - \log(x+1) + \frac{x}{x-1} - \frac{x}{x+1}$$

$$\therefore y_1 = \log(x-1) - \log(x+1) + \frac{(x-1)+1}{x-1} - \frac{(x+1)-1}{x+1}$$

$$\therefore y_1 = \log(x-1) - \log(x+1) + 1 + \frac{1}{x-1} - 1 + \frac{1}{x+1}$$

Changing  $n$  to  $n-1$  for the first two terms, we get

$$\begin{aligned} y_n &= \frac{(-1)^{n-2} (n-2)!}{(x-1)^{n-1}} - \frac{(-1)^{n-2} (n-2)!}{(x+1)^{n-1}} + \frac{(-1)^{n-1} (n-1)!}{(x-1)^n} \\ &\quad + \frac{(-1)^n (n-1)!}{(x+1)^n} \\ &= (-1)^{n-2} (n-2)! \left[ \frac{1}{(x-1)^{n-1}} - \frac{1}{(x+1)^{n-1}} + \frac{(-1)(n-1)}{(x-1)^n} + \frac{(-1)(n-1)}{(x+1)^n} \right] \end{aligned}$$

$$= (-1)^{n-2} (n-2)! \left[ \frac{x-1}{(x-1)^n} - \frac{x+1}{(x+1)^n} + \frac{-n+1}{(x-1)^n} + \frac{-n+1}{(x+1)^n} \right]$$

$$\therefore y_n = (-1)^{n-2} (n-2)! \left[ \frac{x-n}{(x-1)^n} - \frac{x+n}{(x+1)^n} \right]$$



## Example:5

- ❖ Prove that the value of  $n^{\text{th}}$  differential coefficient of  $x^3 / (x^2 - 1)$  for  $x = 0$  is 0 if  $n$  is even and  $-n!$  if  $n$  is odd and greater than 1.

❖ Solution  $y = \frac{x^3}{x^2 - 1} = x + \frac{x}{x^2 - 1}$

$$\therefore y = x + \frac{1}{2} \left[ \frac{1}{x-1} + \frac{1}{x+1} \right]$$

$$\therefore y_n = \frac{1}{2} \left[ \frac{(-1)^n n!}{(x-1)^{n+1}} + \frac{(-1)^n n!}{(x+1)^{n+1}} \right]$$

Putting  $x = 0$ ,  $y_n(0) = \frac{(-1)^n n!}{2} \left[ \frac{1}{(-1)^{n+1}} + \frac{1}{(1)^{n+1}} \right]$

When  $n$  is even,  $(n + 1)$  is odd,

$$\therefore y_n(0) = \frac{(-1)^n n!}{2} [-1 + 1] = 0$$

When  $n$  is odd,  $(n + 1)$  is even,

$$\therefore y_n(0) = \frac{(-1)^n n!}{2} [1 + 1] = -n!$$

# Practice Problems

$$\diamond \frac{x^4}{(x-1)(x-2)}$$

$$\diamond \frac{x^2}{(x-1)(2x+3)}$$

$$\diamond \frac{x}{1-4x^2}$$

$$\diamond \frac{1}{x^4 - a^4}$$

$$\diamond \text{ If } y = x \cot h^{-1} x, \text{ prove that}$$

$$y_n = \frac{(-1)^n (n-2)!}{2} \left[ \frac{x-n}{(x-1)^n} - \frac{x+n}{(x+1)^n} \right].$$

$$\frac{x^2 + 4x + 1}{x^2 + 2x^2 - x - 2}$$

## Example:6

❖ If  $y = \sin rx + \cos rx$  then prove that

$$y_n = r^n [1 + (-1)^n \sin 2rx]^{1/2}$$

❖ **Solution**

$$\begin{aligned} y_n &= r^n \left[ \sin \left( rx + \frac{n\pi}{2} \right) + \cos \left( rx + \frac{n\pi}{2} \right) \right] \\ &= r^n \left[ \left\{ \sin \left( rx + \frac{n\pi}{2} \right) + \cos \left( rx + \frac{n\pi}{2} \right) \right\}^2 \right]^{1/2} \\ &= r^n \left[ \sin^2 \left( rx + \frac{n\pi}{2} \right) + \cos^2 \left( rx + \frac{n\pi}{2} \right) \right. \\ &\quad \left. + 2 \sin \left( rx + \frac{n\pi}{2} \right) \cos \left( rx + \frac{n\pi}{2} \right) \right]^{1/2} \\ &= r^n \left[ 1 + 2 \sin \left( rx + \frac{n\pi}{2} \right) \cdot \cos \left( rx + \frac{n\pi}{2} \right) \right]^{1/2} \end{aligned}$$

$$= r^n \left[ 1 + 2 \sin \left( rx + \frac{n\pi}{2} \right) \cdot \cos \left( rx + \frac{n\pi}{2} \right) \right]^{1/2}$$

$$= r^n \left[ 1 + \sin 2 \left( rx + \frac{n\pi}{2} \right) \right]^{1/2}$$

$$= r^n [1 + \sin(2rx + n\pi)]^{1/2}$$

since  $\sin(n\pi + \theta) = (-1)^n \sin \theta.$

$$= r^n [1 + (-1)^n \sin 2rx]^{1/2}$$

## Example:7

❖ If  $y = \sin^2 x \cos^3 x$  then find  $y_n$

❖ **Solution**  $y = \sin^2 x \cos^2 x \cdot \cos x = \frac{1}{4} (\sin 2x)^2 \cos x$

$$= \frac{1}{8} (1 - \cos 4x) \cos x$$

$$= \frac{1}{8} (\cos x - \cos 4x \cos x)$$

$$= \frac{1}{8} \cos x - \frac{1}{16} [\cos 5x + \cos 3x]$$

$$y_n = \frac{1}{8} \cos \left( x + \frac{n\pi}{2} \right) - \frac{1}{16} \cdot 5^n \cos \left( 5x + \frac{n\pi}{2} \right) \\ - \frac{1}{16} \cdot 3^n \cos \left( 3x + \frac{n\pi}{2} \right)$$

## Example:8

❖ If  $y = 2^x \sin^2 x \cos^3 x$  then find  $y_n$

❖ **Solution:** note that  $2^x = e^{x \log 2} = e^{ax}$  where  $a = \log 2$

$$\therefore \sin^2 x \cos^3 x = \frac{1}{8} \cos x - \frac{1}{16} (\cos 5x + \cos 3x)$$

$$\therefore y = \frac{1}{8} e^{ax} \cos x - \frac{1}{16} e^{ax} \cos 5x - \frac{1}{16} e^{ax} \cos 3x$$

Using formula (11), we get,

$$\begin{aligned} y_n &= \frac{1}{8} r_1^n e^{ax} \cos(x + n\Phi_1) - \frac{1}{16} r_2^n e^{ax} \cos(5x + n\Phi_2) \\ &\quad - \frac{1}{16} r_3^n e^{ax} \cos(3x + n\Phi_3) \\ &= \frac{1}{8} r_1^n 2^x \cos(x + n\Phi_1) - \frac{1}{16} r_2^n 2^x \cos(5x + n\Phi_2) \\ &\quad - \frac{1}{16} r_3^n 2^x \cos(3x + n\Phi_3) \end{aligned}$$

where,  $r_1 = \sqrt{(\log 2)^2 + 1^2},$

$$\Phi_1 = \tan^{-1} \left( \frac{1}{\log 2} \right),$$

$$r_2 = \sqrt{(\log 2)^2 + 5^2}$$

$$\Phi_2 = \tan^{-1} \left( \frac{5}{\log 2} \right),$$

$$r_3 = \sqrt{(\log 2)^2 + 3^2},$$

$$\Phi_3 = \tan^{-1} \left( \frac{3}{\log 2} \right).$$



# Practice Problems

❖ Find  $n$ th derivative of the following functions.

❖  $\sin 2x \sin 3x \cos 4x$

❖  $\sin^3 3x$

❖  $e^x \cos^2 x \cos x$

❖  $2^x \sin^2 x \cos x$

❖  $\cos^4 x$

❖ If  $y = \cos h 2x$ , prove that  
 $y_n = 2^n \sin h 2x$  if  $n$  is odd and  
 $y_n = 2^n \cos h 2x$  if  $n$  is even.



## Example:9

❖ If  $y = \frac{x}{x^2 + a^2}$ , prove that

$$y_n = (-1)^n \cdot n! a^{-n-1} \sin^{n+1} \theta \cos(n+1)\theta \quad \text{where } \theta = \tan^{-1}(a/x).$$

❖ **Solution :**  $y = \frac{x}{x^2 + a^2} = \frac{x}{(x + ai)(x - ai)}$

$$= \frac{1}{2} \left[ \frac{1}{x + ai} + \frac{1}{x - ai} \right] \quad [\text{By partial fractions}]$$

$$y_n = \frac{1}{2} \left[ \frac{(-1)^n n!}{(x + ai)^{n+1}} + \frac{(-1)^n \cdot n!}{(x - ai)^{n+1}} \right]$$

Let  $x = r \cos \theta$ ,  $a = r \sin \theta$ ,  $r^2 = (x^2 + a^2)$  and  $\theta = \tan^{-1}(a/x)$

$$\therefore \frac{1}{(x + ai)^{n+1}} = \frac{1}{r^{n+1} (\cos \theta + i \sin \theta)^{n+1}}$$

$$= \frac{1}{r^{n+1}} \cdot \frac{1}{\cos(n+1)\theta + i \sin(n+1)\theta}$$

By De Moivre's Theorem

$$\therefore \frac{1}{(x + ai)^{n+1}} = \frac{1}{r^{n+1}} \cdot [\cos(n+1)\theta - i \sin(n+1)\theta]$$

And,

$$\begin{aligned} \frac{1}{(x - ai)^{n+1}} &= \frac{1}{r^{n+1} (\cos \theta - i \sin \theta)^{n+1}} \\ &= \frac{1}{r^{n+1}} \cdot \frac{1}{\cos(n+1)\theta - i \sin(n+1)\theta} \\ &= \frac{1}{r^{n+1}} \cdot [\cos(n+1)\theta + i \sin(n+1)\theta] \end{aligned}$$

Adding the two results,

$$\frac{1}{(x - ai)^{n+1}} + \frac{1}{(x + ai)^{n+1}} = \frac{1}{r^{n+1}} \cdot 2 \cos(n+1)\theta$$

$$\therefore y_n = (-1)^n \cdot n! r^{-n-1} \cos(n+1)\theta$$

## Example:10

❖ If  $y = \tan^{-1} x$  then find  $y_n = \frac{(-1)^{n-1}(n-1)!}{(x^2+1)^{\frac{n}{2}}} \sin(n \tan^{-1} \frac{1}{x})$

❖ **Solution:** Differentiating  $y = \tan^{-1} x$ , w.r.t.  $x$ , we get,

$$y_1 = \frac{1}{x^2 + 1} = \frac{1}{(x+i)(x-i)} = \frac{1}{2i} \left[ \frac{1}{(x-i)} - \frac{1}{(x+i)} \right]$$

Differentiating  $(n-1)$  times,

$$y_n = \frac{1}{2i} \left[ \frac{(-1)^{n-1}(n-1)!}{(x-i)^n} - \frac{(-1)^{n-1}(n-1)!}{(x+i)^n} \right] \dots\dots\dots(1)$$

Putting  $r = r \cos \theta$ ,  $1 = r \sin \theta$   $r = \sqrt{1+x^2}$  and  $\theta = \tan^{-1} (1/x)$ ,

$$\frac{1}{(x-i)^n} = \frac{1}{r^n (\cos \theta - i \sin \theta)^n} = \frac{1}{r^n} (\cos n \theta + i \sin n \theta)$$

Similarly, 
$$\frac{1}{(x+i)^n} = \frac{1}{r^n (\cos \theta + i \sin \theta)^n} = \frac{1}{r^n} (\cos n \theta - i \sin n \theta)$$

$$\therefore \frac{1}{(x-i)^n} - \frac{1}{(x+i)^n} = \frac{2i}{r^n} \sin n\theta$$

from (1), we get,

$$\begin{aligned} y_n &= \frac{(-1)^{n-1} (n-1)!}{2i} \cdot \frac{2i}{r^n} \sin n\theta \\ &= (-1)^{n-1} (n-1)! \cdot \frac{1}{r^n} \sin n\theta \end{aligned} \dots\dots\dots(2)$$

Now, we put  $r = \sqrt{1+x^2}$  and  $\theta = \tan^{-1}\left(\frac{1}{x}\right)$  in (2),

$$\therefore y_n = \frac{(-1)^{n-1} (n-1)!}{(x^2+1)^{n/2}} \sin \left[ n \tan^{-1}\left(\frac{1}{x}\right) \right]$$

(HW) **If  $y = \tan^{-1}x$  then Prove that**

$$y_n = (-1)^{n-1} (n-1)! \sin^n \theta \sin n\theta ; \text{ where } \theta = \tan^{-1}\left(\frac{1}{x}\right)$$

**Hint:** In (2) put  $r = \frac{1}{\sin\theta}$

## Example:11

❖ If  $y = \cos^{-1} \left( \frac{x - x^{-1}}{x + x^{-1}} \right)$ , prove that  $y_n = 2 (-1)^{n-1} (n-1)! \sin^n \theta \sin n \theta$   
 where  $\theta = \tan^{-1} (1/x)$ .

❖ **Solution :** Putting  $x = \tan \alpha \quad \therefore \alpha = \tan^{-1} x$ .

$$y = \cos^{-1} \left( \frac{x^2 - 1}{x^2 + 1} \right) = \cos^{-1} \left( \frac{\tan^2 \alpha - 1}{\tan^2 \alpha + 1} \right)$$

$$\therefore y = \cos^{-1} \left[ - \frac{(\cos^2 \alpha - \sin^2 \alpha) / \cos^2 \alpha}{1 / \cos^2 \alpha} \right]$$

$$= \cos^{-1} [ - (\cos^2 \alpha - \sin^2 \alpha) ]$$

$$= \cos^{-1} [ - (\cos 2\alpha) ] = \cos^{-1} \cos (\pi + 2\alpha)$$

$$= \pi + 2\alpha = \pi + 2 \tan^{-1} x$$

$$\therefore y_1 = 2 \cdot \frac{1}{x^2 + 1} \quad (\text{Proceed as per previous example})$$

# Leibnitz's Theorem

❖ If  $u$  and  $v$  are functions of  $x$  such that their  $n^{th}$  derivatives exist, then the  $n^{th}$  derivative of their product is given by

$$(u v)_n = u_n v + n_{C_1} u_{n-1} v_1 + n_{C_2} u_{n-2} v_2 + \cdots + n_{C_r} u_{n-r} v_r + \cdots + u v_n$$

$$(u v)_n = u_n v + n_{C_1} u_{n-1} v_1 + n_{C_2} u_{n-2} v_2 + \cdots + n_{C_r} u_{n-r} v_r + \cdots + u v_n$$

where  $u_r$  and  $v_r$  represent  $r^{th}$  derivatives of  $u$  and  $v$  respectively.

**Remark:** The term which vanishes after differentiating finitely should be taken as  $v$ .



## Example:12

❖ Find the  $n^{th}$  derivative of  $x \log x$

❖ **Solution:** Let  $u = \log x$  and  $v = x$

$\therefore n^{th}$  derivative of  $\log(ax + b)$  is given by  $(-1)^{n-1} \frac{(n-1)! a^n}{(ax+b)^n}$

$$\text{Then } u_n = (-1)^{n-1} \frac{(n-1)!}{x^n} \text{ and } u_{n-1} = (-1)^{n-2} \frac{(n-2)!}{x^{n-1}}$$

Now, by Leibnitz's theorem, we have

$$(u v)_n = u_n v + n_{C_1} u_{n-1} v_1 + n_{C_2} u_{n-2} v_2 + \cdots + n_{C_r} u_{n-r} v_r + \cdots + u v_n$$

$$\Rightarrow (x \log x)_n = (-1)^{n-1} \frac{(n-1)!}{x^n} x + n(-1)^{n-2} \frac{(n-2)!}{x^{n-1}} + 0$$

$$= (-1)^{n-1} \frac{(n-1)!}{x^{n-1}} + n(-1)^{n-2} \frac{(n-2)!}{x^{n-1}}$$

$$= (-1)^{n-2} \frac{(n-2)!}{x^{n-1}} [-(n-1) + n] = (-1)^{n-2} \frac{(n-2)!}{x^{n-1}}$$

## Example:13

❖ If  $y = a \cos(\log x) + b \sin(\log x)$ , show that

$$x^2 y_{n+2} + (2n + 1)xy_{n+1} + n(n + 1)y_n = 0$$

❖ Solution: Here  $y = a \cos(\log x) + b \sin(\log x)$

$$\Rightarrow y_1 = -\frac{a}{x} \sin(\log x) + \frac{b}{x} \cos(\log x)$$

$$\Rightarrow xy_1 = -a \sin(\log x) + b \cos(\log x)$$

Differentiating both sides w.r.t.  $x$ , we get

$$xy_2 + y_1 = -\frac{a}{x} \cos(\log x) + \frac{-b}{x} \sin(\log x)$$

$$\Rightarrow x^2 y_2 + xy_1 = -\{a \cos(\log x) + b \sin(\log x)\} = -y$$

$$\Rightarrow x^2 y_2 + xy_1 + y = 0$$



Using Leibnitz's theorem, we get

$$\begin{aligned} & (y_{n+2}x^2 + n_{C_1}y_{n+1}2x + n_{C_2}y_n \cdot 2) + (y_{n+1}x + n_{C_1}y_n \cdot 1) + y_n = 0 \\ \Rightarrow & y_{n+2}x^2 + y_{n+1}2nx + n(n-1)y_n + y_{n+1}x + ny_n + y_n = 0 \\ \Rightarrow & x^2y_{n+2} + (2n+1)xy_{n+1} + (n^2+1)y_n = 0 \end{aligned}$$

## Example:14

❖ If  $y = \log(x + \sqrt{1 + x^2})$ , prove that

$$(1 + x^2)y_{n+2} + (2n + 1)xy_{n+1} + n^2y_n = 0$$

❖ Solution:  $y = \log(x + \sqrt{1 + x^2})$

$$\Rightarrow y_1 = \frac{1}{x + \sqrt{1 + x^2}} \left( 1 + \frac{1}{2\sqrt{1 + x^2}} 2x \right) = \frac{1}{\sqrt{1 + x^2}}$$

$$\Rightarrow (1 + x^2)y_1^2 = 1$$

Differentiating both sides w.r.t.  $x$ , we get

$$(1 + x^2)2y_1y_2 + 2xy_1^2 = 0$$

$$\Rightarrow (1 + x^2)y_2 + xy_1 = 0$$

Using Leibnitz's theorem

$$[y_{n+2}(1+x^2) + n_{C_1}y_{n+1}2x + n_{C_2}y_n \cdot 2] + (y_{n+1}x + n_{C_1}y_n \cdot 1) = 0$$

$$\Rightarrow y_{n+2}(1+x^2) + y_{n+1}2nx + n(n-1)y_n + y_{n+1}x + ny_n = 0$$

$$\Rightarrow (1+x^2)y_{n+2} + (2n+1)xy_{n+1} + n^2y_n = 0$$

## Example:15

- ❖ If  $y = \sin(m \sin^{-1} x)$ , show that  
 $(1 - x^2)y_{n+2} = (2n + 1)xy_{n+1} + (n^2 - m^2)y_n$ . Also find  $y_n(0)$

❖ **Solution:**

$$\text{Here } y = \sin(m \sin^{-1} x) \quad \dots \textcircled{1}$$

$$\Rightarrow y_1 = \frac{m}{\sqrt{1-x^2}} \cos(m \sin^{-1} x) \quad \dots \textcircled{2}$$

$$\Rightarrow (1 - x^2)y_1^2 = m^2 \cos^2(m \sin^{-1} x)$$

$$\Rightarrow (1 - x^2)y_1^2 = m^2 [1 - \sin^2(m \sin^{-1} x)]$$

$$\Rightarrow (1 - x^2)y_1^2 = m^2 (1 - y^2) \quad \dots \textcircled{3}$$

$$\Rightarrow (1 - x^2)y_1^2 + m^2 y^2 = m^2$$

Differentiating w.r.t.  $x$ , we get

$$(1 - x^2)2y_1y_2 + y_1^2(-2x) + m^22yy_1 = 0$$

$$\Rightarrow (1 - x^2)y_2 - xy_1 + m^2y = 0$$

Using Leibnitz's theorem, we get

$$[y_{n+2}(1 - x^2) + n_{c_1}y_{n+1}(-2x) + n_{c_2}y_n(-2)] - (y_{n+1}x + n_{c_1}y_n1) + m^2y_n = 0$$

$$\Rightarrow y_{n+2}(1 - x^2) - y_{n+1}2nx - n(n - 1)y_n - (y_{n+1}x + ny_n) + m^2y_n = 0$$

$$\Rightarrow (1 - x^2)y_{n+2} = (2n + 1)xy_{n+1} + (n^2 - m^2)y_n \quad \dots \textcircled{4}$$

Putting  $x = 0$  in  $\textcircled{1}$ ,  $\textcircled{2}$  and  $\textcircled{3}$

$$y(0) = 0, y_1(0) = m \text{ and } y_2(0) = 0$$

Putting  $x = 0$  in  $\textcircled{4}$ , we get

$$y_{n+2}(0) = (n^2 - m^2)y_n(0)$$

Putting  $n = 1, 2, 3 \dots$  in the above equation, we get

$$y_3(0) = (1^2 - m^2)y_1(0) = (1^2 - m^2)m \quad \because y_1(0) = m$$

$$y_4(0) = (2^2 - m^2)y_2(0) = 0 \quad \because y_2(0) = 0$$

$$y_5(0) = (3^2 - m^2)y_3(0) = m(1^2 - m^2)(3^2 - m^2)$$

$$\Rightarrow y_n(0) = \begin{cases} 0, & \text{if } n \text{ is even} \\ m(1^2 - m^2)(3^2 - m^2) \dots [(n-2)^2 - m^2], & \text{if } n \text{ is odd} \end{cases}$$

# Practice Problems

1. Find  $y_n$ , if  $y = x^3 \cos x$
2. Find  $y_n$ , if  $y = x^2 e^x \cos x$
3. If  $y^{\frac{1}{m}} + y^{\frac{-1}{m}} = 2x$ , prove that  $(x^2 - 1)y_{n+2} + (2n + 1)xy_{n+1} + (n^2 - m^2)y_n = 0$
4. If  $y\sqrt{1+x^2} = \log(x + \sqrt{1+x^2})$ , prove that  $(1+x^2)y_{n+2} + (2n+3)xy_{n+1} + (n+1)^2y_n = 0$
5. If  $y = [x + \sqrt{1+x^2}]^m$ , prove that  $(x^2 + 1)y_{n+2} + (2n+1)xy_{n+1} + (n^2 - m^2)y_n = 0$
6. If  $y = (\sinh^{-1}x)^2$ , show that  $(1+x^2)y_{n+2} + (2n+1)xy_{n+1} + n^2y_n = 0$ . Also find  $y_n(0)$ .
7. If  $y = \cos(m \sin^{-1}x)$ , show that  $(1-x^2)y_{n+2} = (2n+1)xy_{n+1} + (n^2 - m^2)y_n$ . Also find  $y_n(0)$ .
8. If  $f(x) = \tan x$ , prove that  $f^n(0) - n_{C_2}f^{n-2}(0) + n_{C_4}f^{n-4}(0) - \dots = \sin \frac{n\pi}{2}$